Mostly prove term mostly cartesian

theories/Category.v
@@ -25,13 +25,16 @@ Implicit Types X Y: cvar.
 Implicit Type σ: store.
 
 Module Import Hor.
-  Definition Hor t t' := Term.oftype (cons (0, t) nil) t'.
+  #[local]
+  Definition X: vvar := 0.
+
+  Definition Hor t t' := Term.oftype (cons (X, t) nil) t'.
 
   #[program]
-  Definition id t: Hor t t := v_var 0.
-  Next Obligation.
-    repeat constructor.
-  Defined.
+  Definition id t: Hor t t := v_var X.
+
+  #[program]
+  Definition compose {A B C} (f: Hor B C) (g: Hor A B): Hor A C := subst_term g X f.
 
   #[local]
    Lemma shadow:
@@ -47,17 +50,9 @@ Module Import Hor.
     all: try econstructor.
     all: try eauto.
     inversion H1.
-    - subst.
-      constructor.
-    - subst.
-      constructor.
-      all: auto.
-      constructor.
-      all: auto.
+    all: repeat constructor.
+    all: auto.
   Qed.
-
-  #[program]
-  Definition compose {A B C} (f: Hor B C) (g: Hor A B): Hor A C := subst_term g 0 f.
 
   Next Obligation.
   Proof.
@@ -68,6 +63,168 @@ Module Import Hor.
     apply shadow.
     auto.
   Defined.
+
+  Next Obligation.
+    repeat constructor.
+  Defined.
+
+  Lemma compose_id_left {A B} (f: Hor A B): compose (id _) f == f.
+  Proof.
+    destruct f as [f ?].
+    cbn.
+    unfold compose, id.
+    cbn.
+    intros ? H.
+    cbn.
+    destruct (Term.normalize (Term.msubst_preserve H j)) as [N ?].
+    exists N.
+    cbn.
+    split.
+    all: auto.
+  Qed.
+
+  Lemma compose_id_right {A B} (f: Hor A B): compose f (id _) == f.
+  Proof.
+    destruct f as [f ?].
+    cbn.
+    intros ? H.
+    cbn.
+    rewrite Term.subst_var.
+    destruct (Term.normalize (Term.msubst_preserve H j)) as [N ?].
+    exists N.
+    split.
+    all: auto.
+  Qed.
+
+  Lemma compose_assoc {A B C D} (f: Hor C D) (g: Hor B C) (h: Hor A B):
+    compose f (compose g h) == compose (compose f g) h.
+  Proof.
+    destruct f as [f ?], g as [g ?], h as [h ?].
+    cbn.
+    intros ? H.
+    cbn.
+    eset (N := @Term.normalize (msubst p (subst_term (subst_term h X g) X f)) D _).
+    destruct N as [N ?].
+    Unshelve.
+    2: {
+      eapply Term.msubst_preserve.
+      1: eauto.
+      eapply Term.subst_preserve.
+      2: apply shadow; eauto.
+      eapply Term.subst_preserve.
+      2: apply shadow; eauto.
+      auto.
+    }
+    exists N.
+    split.
+    1: auto.
+    rewrite <- Term.subst_assoc.
+    auto.
+  Qed.
+
+  #[program]
+  Definition tt A: Hor A t_unit := v_tt.
+
+  #[program]
+   Definition fanout {A B C} (f: Hor C A) (g: Hor C B): Hor C (A * B) := v_fanout f g.
+
+  #[program]
+  Definition fst {A B}: Hor (A * B) A := v_fst (v_var X).
+
+  #[program]
+  Definition snd {A B}: Hor (A * B) B := v_snd (v_var X).
+
+  Next Obligation.
+  Proof.
+    destruct f as [f ?], g as [g ?].
+    cbn.
+    constructor.
+    all: auto.
+  Defined.
+
+  Next Obligation.
+  Proof.
+    repeat econstructor.
+  Defined.
+
+  Next Obligation.
+  Proof.
+    repeat econstructor.
+  Defined.
+
+  Next Obligation.
+  Proof.
+    repeat econstructor.
+  Defined.
+
+  (* Prove a strict terminal object *)
+  Lemma compose_tt {A B} (f: Hor A B): compose (tt _) f == tt _.
+  Proof.
+    cbn.
+    destruct f as [f ?].
+    intros p ?.
+    cbn.
+    eset (N := @Term.normalize (msubst p v_tt) t_unit _).
+    destruct N as [N ?].
+    Unshelve.
+    2: {
+      eapply Term.msubst_preserve.
+      all: eauto.
+      constructor.
+    }
+    exists N.
+    split.
+    all: auto.
+  Qed.
+
+  Lemma fst_fanout {C A B} (f: Hor C A) (g: Hor C B): compose fst (fanout f g) == f.
+  Proof.
+    destruct f as [f ?], g as [g ?].
+    intros p ?.
+    cbn.
+    eset (N := @Term.normalize (msubst p f) A _).
+    destruct N as [N ?].
+    Unshelve.
+    2: {
+      eapply Term.msubst_preserve.
+      all: eauto.
+    }
+    destruct (Term.normalize (Term.msubst_preserve H j0)).
+    exists N.
+    split.
+    all: auto.
+    rewrite Term.msubst_fst.
+    rewrite Term.msubst_fanout.
+    econstructor.
+    econstructor.
+    1: auto.
+    apply H1.
+  Qed.
+
+  Lemma snd_fanout {C A B} (f: Hor C A) (g: Hor C B): compose snd (fanout f g) == g.
+  Proof.
+    destruct f as [f ?], g as [g ?].
+    intros p ?.
+    cbn.
+    eset (N := @Term.normalize (msubst p g) B _).
+    destruct N as [N ?].
+    Unshelve.
+    2: {
+      eapply Term.msubst_preserve.
+      all: eauto.
+    }
+    destruct (Term.normalize (Term.msubst_preserve H j)).
+    exists N.
+    split.
+    all: auto.
+    rewrite Term.msubst_snd.
+    rewrite Term.msubst_fanout.
+    econstructor.
+    econstructor.
+    1: auto.
+    apply H1.
+    auto.
+  Qed.
 End Hor.
 
 Module Import Vert.
